Bdd/Apply.lean
@@ -1,0 +1,178 @@
+import Bdd.Basic
+import Bdd.Reduce
+-- import Std.HashMap.Basic
+
+open List renaming Vector → Vec
+
+namespace Apply
+inductive RawPointer where
+  | terminal : Bool → RawPointer
+  | node     : Nat  → RawPointer
+
+structure RawNode (n) where
+  var  : Fin n
+  low  : RawPointer
+  high : RawPointer
+
+abbrev p2t : Nat → Nat → Nat := fun l r ↦ (l + 2) * (r + 2)
+
+structure State (n) (m) (m') where
+  cache : Std.HashMap (Pointer m × Pointer m') (Pointer (p2t m m'))
+  heap : Vec (Node n (p2t m m')) (p2t m m')
+  next : Fin (p2t m m')
+
+-- def threeval (op : (Bool → Bool → Bool)): Pointer m → Pointer m' → (Option Bool)
+--   | .terminal b => fun
+--     | .terminal b' => op b b'
+--     | .node _ => if (op b false) = (op b true) then some (op b false) else none
+--   | .node _ => fun
+--     | .terminal b' => if (op false b') = (op true b') then some (op false b') else none
+--     | .node _ => none
+
+-- def apply_helper (nid : Fin (m * m')) (heap : Vec (Node n (m * m')) (m * m')) (cache : Std.HashMap (Pointer m × Pointer m') (Pointer (m * m'))) (op : (Bool → Bool → Bool)) (O : OBdd n m) (U : OBdd n' m') :
+--     Bdd n (m * m') :=
+--   match cache.get? ⟨O.1.root, U.1.root⟩ with
+--   | some root => ⟨heap, root⟩
+--   | none =>
+--     if (threeval op O.1.root U.1.root) = none
+--     then
+--       sorry
+--     else sorry
+
+-- def apply_helper {n m m' : Nat} (op : (Bool → Bool → Bool)) (O : OBdd n m.succ) (U : OBdd n' m'.succ) :
+--     StateM (State n m.succ m'.succ) (Pointer (m.succ * m'.succ)) := do
+--   let s ← get
+--   match s.cache.get? ⟨O.1.root, U.1.root⟩ with
+--   | some root => pure root
+--   | none =>
+--     match threeval op O.1.root U.1.root with
+--     | some b =>
+--       set (⟨s.cache.insert ⟨O.1.root, U.1.root⟩ (.terminal b), s.heap, s.next⟩ : State n m.succ m'.succ)
+--       pure (.terminal b)
+--     | none =>
+--       if O.var ≤ U.var
+--       then
+--         if O.var ≥ U.var
+--         then
+-- --        set (⟨s.cache.insert ⟨O.1.root, U.1.root⟩ (.node s.next), s.heap.set s.next sorry, s.next + 1⟩ : State n m.succ m'.succ)
+--           pure (.node s.next)
+--         else sorry
+--       else sorry
+
+def cache_get {n m m' : Nat} (O_root : Pointer m) (U_root : Pointer m') :
+    StateM (State n m m') (Option (Pointer (p2t m m'))) := fun s ↦
+  ⟨(s.cache.get? ⟨O_root, U_root⟩), s⟩
+
+def cache_put {n m m' : Nat} (O_root : Pointer m) (U_root : Pointer m') (val : Pointer (p2t m m')) :
+    StateM (State n m m') Unit := fun s ↦
+  ⟨(), ⟨s.cache.insert ⟨O_root, U_root⟩ val, s.heap, s.next⟩⟩
+
+def heap_push {n m m' : Nat} (N : Node n (p2t m m')) :
+    StateM (State n m m') Unit := fun s ↦
+  ⟨(), ⟨s.cache, s.heap.set s.next N, s.next + 1⟩⟩
+
+def next : StateM (State n m m') (Fin (p2t m m')) := do
+  let s ← get
+  pure s.next
+
+def apply_helper {n m m' : Nat} (op : (Bool → Bool → Bool)) (O : OBdd n m) (U : OBdd n m') :
+    StateM (State n m m') (Pointer (p2t m m')) := do
+  let cache_hit ← cache_get O.1.root U.1.root
+  match cache_hit with
+  | some root => pure root
+  | none =>
+    match O_root_def : O.1.root with
+    | .terminal b =>
+      match U_root_def : U.1.root with
+      | .terminal b' =>
+        let b'' := op b b'
+        cache_put O.1.root U.1.root (.terminal b'')
+        pure (.terminal b'')
+      | .node j' =>
+        let l ← apply_helper op O (U.low  U_root_def)
+        let h ← apply_helper op O (U.high U_root_def)
+        let nid ← next
+        cache_put O.1.root U.1.root (.node nid)
+        heap_push ⟨U.1.heap[j'].var, l, h⟩
+        pure (.node nid)
+    | .node j =>
+      match U_root_def : U.1.root with
+      | .terminal b' =>
+        let l ← apply_helper op (O.low  O_root_def) U
+        let h ← apply_helper op (O.high O_root_def) U
+        let nid ← next
+        cache_put O.1.root U.1.root (.node nid)
+        heap_push ⟨O.1.heap[j].var, l, h⟩
+        pure (.node nid)
+      | .node j' =>
+        if O.1.heap[j].var < U.1.heap[j'].var
+        then
+          let l ← apply_helper op (O.low  O_root_def) U
+          let h ← apply_helper op (O.high O_root_def) U
+          let nid ← next
+          cache_put O.1.root U.1.root (.node nid)
+          heap_push ⟨O.1.heap[j].var, l, h⟩
+          pure (.node nid)
+        else
+          if O.1.heap[j].var > U.1.heap[j'].var
+          then
+            let l ← apply_helper op O (U.low  U_root_def)
+            let h ← apply_helper op O (U.high U_root_def)
+            let nid ← next
+            cache_put O.1.root U.1.root (.node nid)
+            heap_push ⟨U.1.heap[j'].var, l, h⟩
+            pure (.node nid)
+          else
+            let l ← apply_helper op (O.low  O_root_def) (U.low  U_root_def)
+            let h ← apply_helper op (O.high O_root_def) (U.high U_root_def)
+            let nid ← next
+            cache_put O.1.root U.1.root (.node nid)
+            heap_push ⟨U.1.heap[j'].var, l, h⟩
+            pure (.node nid)
+termination_by (O, U)
+decreasing_by
+  · right; exact oedge_of_low
+  · right; exact oedge_of_high
+  · left;  exact oedge_of_low
+  · left;  exact oedge_of_high
+  · left;  exact oedge_of_low
+  · left;  exact oedge_of_high
+  · right; exact oedge_of_low
+  · right; exact oedge_of_high
+  · left;  exact oedge_of_low
+  · left;  exact oedge_of_high
+
+def apply {n m m' : Nat} : (Bool → Bool → Bool) → OBdd n.succ m → OBdd n.succ m' → Bdd n.succ (p2t m m') := fun op O U ↦
+  let ⟨root, state⟩ := apply_helper op O U ⟨Std.HashMap.empty, Vec.replicate _ ⟨0, .terminal false, .terminal false⟩, 0⟩
+  ⟨state.heap, root⟩
+
+theorem apply_spec {n m m' : Nat} {op : (Bool → Bool → Bool)} {O : OBdd n.succ m} {U : OBdd n.succ m'} : ∃ (o : Bdd.Ordered (apply op O U)), ∀ I, (op (O.evaluate I) (U.evaluate I)) = OBdd.evaluate ⟨apply op O U, o⟩ I := by
+  sorry
+
+end Apply
+
+def Bdd.fromVar {n} : Fin n → Bdd n 1 := fun i ↦ ⟨⟨[⟨i, .terminal false, .terminal true⟩], rfl⟩, .node 0⟩
+
+lemma Bdd.fromVar_Ordered {n} {i : Fin n} : Bdd.Ordered (fromVar i) := by
+  apply Ordered_of_Proper
+  simp only [fromVar, Proper]
+  simp only [Vec.instMembership, Function.comp_apply, List.Vector.toList_singleton, List.mem_cons, List.not_mem_nil, or_false, forall_eq]
+  intro j contra
+  cases contra <;> contradiction
+
+def foo := Compactify.compactify' ⟨(Reduce.reduce ⟨(Apply.apply Bool.and ⟨(Bdd.fromVar (n := 2) 0), Bdd.fromVar_Ordered⟩ ⟨(Bdd.fromVar (n := 2) 1), Bdd.fromVar_Ordered⟩), Apply.apply_spec.1⟩), Reduce.reduce_spec.1⟩
+def bar := Compactify.compactify' ⟨(Reduce.reduce ⟨(Apply.apply Bool.or ⟨(Bdd.fromVar (n := 3) 0), Bdd.fromVar_Ordered⟩ ⟨(Bdd.fromVar (n := 3) 1), Bdd.fromVar_Ordered⟩), Apply.apply_spec.1⟩), Reduce.reduce_spec.1⟩
+def baz := Compactify.compactify' ⟨(Reduce.reduce ⟨(Apply.apply Bool.or (⟨(Apply.apply Bool.and example_bdd example_bdd), Apply.apply_spec.1⟩) example_bdd), sorry⟩), sorry⟩
+
+#eval! baz
+#eval! foo
+#eval! bar
+
+#eval (Bdd.fromVar (n := 2) 0)
+#eval Apply.apply Bool.and ⟨(Bdd.fromVar (n := 2) 0), Bdd.fromVar_Ordered⟩ ⟨(Bdd.fromVar (n := 2) 1), Bdd.fromVar_Ordered⟩
+#eval! Reduce.reduce ⟨(Apply.apply Bool.and ⟨(Bdd.fromVar (n := 2) 0), Bdd.fromVar_Ordered⟩ ⟨(Bdd.fromVar (n := 2) 1), Bdd.fromVar_Ordered⟩), Apply.apply_spec.1⟩
+#eval! Compactify.compactify' ⟨(Reduce.reduce ⟨(Apply.apply Bool.and ⟨(Bdd.fromVar (n := 2) 0), Bdd.fromVar_Ordered⟩ ⟨(Bdd.fromVar (n := 2) 1), Bdd.fromVar_Ordered⟩), Apply.apply_spec.1⟩), Reduce.reduce_spec.1⟩
+#eval! Compactify.compactify' ⟨(Reduce.reduce ⟨(Apply.apply Bool.or ⟨(Bdd.fromVar (n := 2) 0), Bdd.fromVar_Ordered⟩ ⟨(Bdd.fromVar (n := 2) 1), Bdd.fromVar_Ordered⟩), Apply.apply_spec.1⟩), Reduce.reduce_spec.1⟩
+
+
+#eval! Compactify.compactify' ⟨(Apply.apply Bool.and ⟨(Bdd.fromVar (n := 2) 0), Bdd.fromVar_Ordered⟩ ⟨(Bdd.fromVar (n := 2) 1), Bdd.fromVar_Ordered⟩), Apply.apply_spec.1⟩
